theories/TypeSafety.v
@@ -3,6 +3,7 @@ From Lang Require Import
   Terms
   Types.
 
+(*
 Theorem no_type_in_type : forall ctx,
   ~Typed ctx TmStar TmStar.
 Proof.
@@ -11,7 +12,6 @@ Proof.
   (* inversion C. subst. apply IHC; reflexivity. *)
 Qed.
 
-(*
 Theorem BAD_exists_term_typed_void : exists t,
   Typed [] t TmVoid.
 Proof.
